theories/case_studies/multiuser_kvs/kvs_spec_getFullKey.v
@@ -1,9 +1,9 @@
 From iris.proofmode Require Import proofmode.
-From griotte Require Import logrel rules.
-From griotte Require Import switcher kvs.
 From griotte Require Import proofmode.
-From griotte Require Export kvs_preamble.
+From griotte Require Import logrel rules.
 From griotte Require Import wp_rules_interp.
+From griotte Require Import switcher kvs.
+From griotte Require Export kvs_preamble.
 
 Section KVS_getFullKey.
   Context
